theories/examples/switcher/switcher_spec.v
@@ -8,6 +8,7 @@ Section Switcher.
     {Σ:gFunctors}
     {ceriseg:ceriseG Σ} {sealsg: sealStoreG Σ}
     {Cname : CmptNameG}
+    {switcherg :switcherG}
     {stsg : STSG Addr region_type Σ} {heapg : heapGS Σ}
     {nainv: logrel_na_invs Σ}
     `{MP: MachineParameters}.
