theories/ftlr/JmpCap.v
@@ -11,6 +11,7 @@ Section fundamental.
     {Σ:gFunctors}
     {ceriseg:ceriseG Σ} {sealsg: sealStoreG Σ}
     {Cname : CmptNameG}
+    {switcherg :switcherG}
     {stsg : STSG Addr region_type Σ} {heapg : heapGS Σ}
     {nainv: logrel_na_invs Σ}
     `{MP: MachineParameters}.
@@ -79,14 +80,26 @@ Section fundamental.
           iEval (rewrite fixpoint_interp1_eq) in "Hwsrc".
           simpl; rewrite /enter_cond.
           iDestruct "Hwsrc" as "#H".
-          iAssert (future_world g0 W W) as "Hfuture".
-          { iApply futureworld_refl. }
-          iSpecialize ("H" with "Hfuture").
-          iDestruct "H" as "[H _]".
-          iDestruct (region_close with "[$Hstate $Hr Hw $Ha $HmonoV]") as "Hr"; eauto.
-          { destruct ρ;auto;[|ospecialize (Hnotfrozen _)];contradiction. }
-          iDestruct ("H" with "[$Hmap $Hr $Hsts $Hown]") as "HA"; eauto.
-          iFrame "#%".
+          destruct ( decide (WCap (E rx pw dl dro) g0 b0 e0 a0 = switcher_ret_entry_point) ) as [? |?].
+          * rewrite (decide_True ( P:= (_ = switcher_ret_entry_point))); last done.
+            rewrite switcher_ret_correct in e1; simplify_eq.
+            iAssert (future_world Local W W) as "Hfuture".
+            { iApply futureworld_refl. }
+            iSpecialize ("H" with "Hfuture").
+            iDestruct "H" as "[H _]".
+            iDestruct (region_close with "[$Hstate $Hr Hw $Ha $HmonoV]") as "Hr"; eauto.
+            { destruct ρ;auto;[|ospecialize (Hnotfrozen _)];contradiction. }
+            iDestruct ("H" with "[$Hmap $Hr $Hsts $Hown]") as "HA"; eauto.
+            iFrame "#%".
+          * rewrite (decide_False ( P:= (_ = switcher_ret_entry_point))); last done.
+            iAssert (future_world g0 W W) as "Hfuture".
+            { iApply futureworld_refl. }
+            iSpecialize ("H" with "Hfuture").
+            iDestruct "H" as "[H _]".
+            iDestruct (region_close with "[$Hstate $Hr Hw $Ha $HmonoV]") as "Hr"; eauto.
+            { destruct ρ;auto;[|ospecialize (Hnotfrozen _)];contradiction. }
+            iDestruct ("H" with "[$Hmap $Hr $Hsts $Hown]") as "HA"; eauto.
+            iFrame "#%".
         + (* case p1 ≠ E *)
           iEval (rewrite fixpoint_interp1_eq) in "Hinv_interp".
           iNext; iIntros "_".
