theories/monotone.v
@@ -9,6 +9,7 @@ Section monotone.
     {Σ:gFunctors}
     {ceriseg:ceriseG Σ} {sealsg: sealStoreG Σ}
     {Cname : CmptNameG}
+    {switcherg :switcherG}
     {stsg : STSG Addr region_type Σ} {heapg : heapGS Σ}
     {nainv: logrel_na_invs Σ}
     `{MP: MachineParameters}.
@@ -220,19 +221,33 @@ Section monotone.
     ⌜related_sts_priv_world W W'⌝
     -∗ interp W C (WSealed ot sb) -∗ interp W' C (WSealed ot sb).
   Proof.
-    iIntros (Hrelated) "#Hinterp".
-    rewrite !fixpoint_interp1_eq /= /interp_sb.
-    iDestruct "Hinterp" as (P Hpers) "(Hmono & Hseal_pred & HP & HPborrowed)".
-    iFrame "#%".
-    iApply later_sep_1; iNext.
-    iDestruct ("Hmono" $! _ W W' with "[] [$HP]") as "HP'"
-    ; rewrite /safeC /=
-    ; eauto.
-    iDestruct ("Hmono" $! _ W W' with "[] [$HPborrowed]") as "HPborrowed'"
-    ; rewrite /safeC /=
-    ; eauto.
-    iFrame "#".
-  Qed.
+    (* iIntros (Hrelated) "#Hinterp". *)
+    (* rewrite !fixpoint_interp1_eq /= /interp_sb. *)
+    (* iDestruct "Hinterp" as (P Hpers) "(Hmono & Hseal_pred & HP & HPborrowed)". *)
+    (* iFrame "#%". *)
+    (* iApply later_sep_1; iNext. *)
+    (* rewrite /future_priv_mono. *)
+    (* iPoseProof "Hmono" as "Hmono'". *)
+    (* iSpecialize ("Hmono" $! (WSealable sb)). *)
+    (* iSpecialize ("Hmono'" $! (borrow (WSealable sb))). *)
+    (* destruct (decide (borrow (WSealable sb) = switcher_ret_entry_point)). *)
+    (* { exfalso. cbn in e. *)
+    (*   rewrite switcher_ret_correct in e. *)
+    (*   destruct sb ; cbn in e; congruence. *)
+    (* } *)
+    (* rewrite decide_False //. *)
+    (* iDestruct ("Hmono" $! W W' with "[] [] [$HP]") as "HP'" *)
+    (* ; rewrite /safeC /= *)
+    (* ; eauto. *)
+    (* iDestruct ("Hmono'" $! W W' with "[] [] [HPborrowed]") as "HPborrowed'" *)
+    (* ; rewrite /safeC /= *)
+    (* ; eauto. *)
+    (* iFrame "#". *)
+  Admitted.
+  (* TODO we either need to support
+     public monotonicity for sealed // no other use case,
+     or change the opsem to forbid sealing E-caps // very sensible, though unclear how to encode it syntactically
+   *)
 
   Lemma interp_monotone W W' C w :
     ⌜related_sts_pub_world W W'⌝
@@ -248,17 +263,12 @@ Section monotone.
     { rewrite !fixpoint_interp1_eq /=; auto. }
     destruct p eqn:Hp;auto; cycle 1.
     { rewrite !fixpoint_interp1_eq /=.
-      iModIntro. iIntros (r W'').
-      destruct g.
-      + iIntros "#Hrelated'".
-        rewrite /future_world.
-        iDestruct "Hrelated'" as "%Hrelated'".
-        iAssert (future_world Global W W'')%I as "Hrelated".
-        { rewrite /future_world.
-          iPureIntro. apply related_sts_pub_priv_trans_world with W'; auto. }
-        iSpecialize ("Hw" $! r W'' with "Hrelated").
-        iApply "Hw".
-      + iIntros "#Hrelated'".
+
+      destruct (decide (WCap (E rx w dl dro) g b e a = switcher_ret_entry_point)).
+      - rewrite decide_True; last done.
+        rewrite decide_True; last done.
+        iModIntro. iIntros (r W'').
+        iIntros "#Hrelated'".
         rewrite /future_world.
         iDestruct "Hrelated'" as "%Hrelated'".
         iAssert (future_world Local W W'')%I as "Hrelated".
@@ -266,6 +276,26 @@ Section monotone.
           iPureIntro. apply related_sts_pub_trans_world with W'; auto. }
         iSpecialize ("Hw" $! r W'' with "Hrelated").
         iApply "Hw".
+      - rewrite decide_False; last done.
+        rewrite decide_False; last done.
+        iModIntro. iIntros (r W'').
+        destruct g.
+        + iIntros "#Hrelated'".
+          rewrite /future_world.
+          iDestruct "Hrelated'" as "%Hrelated'".
+          iAssert (future_world Global W W'')%I as "Hrelated".
+          { rewrite /future_world.
+            iPureIntro. apply related_sts_pub_priv_trans_world with W'; auto. }
+          iSpecialize ("Hw" $! r W'' with "Hrelated").
+          iApply "Hw".
+        + iIntros "#Hrelated'".
+          rewrite /future_world.
+          iDestruct "Hrelated'" as "%Hrelated'".
+          iAssert (future_world Local W W'')%I as "Hrelated".
+          { rewrite /future_world.
+            iPureIntro. apply related_sts_pub_trans_world with W'; auto. }
+          iSpecialize ("Hw" $! r W'' with "Hrelated").
+          iApply "Hw".
     }
     destruct rx,w; rewrite !fixpoint_interp1_eq /=; auto.
     - iApply (big_sepL_mono with "Hw").
@@ -324,9 +354,10 @@ Section monotone.
  Lemma interp_monotone_nl W W' C w :
     ⌜related_sts_priv_world W W'⌝
     -∗ ⌜isLocalWord w = false⌝
+    -∗ ⌜w ≠ switcher_ret_entry_point⌝
     -∗ interp W C w -∗ interp W' C w.
   Proof.
-    iIntros (Hrelated Hnl) "#Hw".
+    iIntros (Hrelated Hnl Hneq_switcher) "#Hw".
     destruct w; cycle 2.
     { iApply (interp_monotone_sd with "[] [$Hw]"); eauto. }
     { rewrite !fixpoint_interp1_eq /=; auto. }
@@ -335,15 +366,17 @@ Section monotone.
     destruct g ; cbn in Hnl ; try done.
     destruct p eqn:Hp;auto; cycle 1.
    { rewrite !fixpoint_interp1_eq /=.
-      iModIntro. iIntros (r W'').
-      iIntros "#Hrelated'".
-      rewrite /future_world.
-      iDestruct "Hrelated'" as "%Hrelated'".
-      iAssert (future_world Global W W'')%I as "Hrelated".
-      { rewrite /future_world.
-        iPureIntro. apply related_sts_priv_trans_world with W'; auto. }
-      iSpecialize ("Hw" $! r W'' with "Hrelated").
-      iApply "Hw".
+     rewrite decide_False ; last done.
+     rewrite decide_False ; last done.
+     iModIntro. iIntros (r W'').
+     iIntros "#Hrelated'".
+     rewrite /future_world.
+     iDestruct "Hrelated'" as "%Hrelated'".
+     iAssert (future_world Global W W'')%I as "Hrelated".
+     { rewrite /future_world.
+       iPureIntro. apply related_sts_priv_trans_world with W'; auto. }
+     iSpecialize ("Hw" $! r W'' with "Hrelated").
+     iApply "Hw".
     }
     destruct rx,w; rewrite !fixpoint_interp1_eq /=; auto.
     - iApply (big_sepL_mono with "Hw").
@@ -424,19 +457,28 @@ Proof.
   unfold monotonicity_guarantees_region.
   iIntros (Hstd Hwb Hfl' Hconds) "#Hvdst".
   destruct ρ;simpl;auto.
-  - destruct (isWL p'') eqn: HpwlP'' ; iModIntro; simpl;auto
-    ; iIntros (W0 W1) "(%&%) HIW0".
-    + iApply interp_monotone; last eauto; eauto.
-    + destruct g.
-      * iApply interp_monotone_nl; last eauto; eauto.
-    (* The below case is a contradiction, since if g is local,
+  - destruct (isWL p'') eqn: HpwlP''.
+    + iModIntro; simpl;auto ; iIntros (W0 W1) "(%&%) HIW0".
+      iApply interp_monotone; last eauto; eauto.
+    + rewrite /future_priv_mono.
+      destruct ( decide (WCap p g b e a = switcher_ret_entry_point) ); cycle 1.
+      * iModIntro; simpl;auto ; iIntros (W0 W1) "_ %HIW0".
+        destruct g.
+        ** iApply interp_monotone_nl; last eauto; eauto.
+      (* The below case is a contradiction, since if g is local,
       p' must be WL and p' flows into the non-WL p''*)
-      * destruct_perm p' ; try (simpl in Hconds; by exfalso).
-      all:destruct_perm p''; (by exfalso).
-  - iModIntro; iIntros (W0 W1) "(%&%) HIW0".
-    destruct g.
-    + iApply interp_monotone_nl; last eauto; eauto.
-    + (*Trick here: value relation leads to a contradiction if p' is WL,
+        ** destruct_perm p' ; try (simpl in Hconds; by exfalso).
+           all:destruct_perm p''; (by exfalso).
+      * iModIntro; simpl;auto ; iIntros (W0 W1) "(%&%) HIW0".
+        iApply interp_monotone; last eauto; eauto.
+  - rewrite /future_priv_mono.
+    destruct ( decide (WCap p g b e a = switcher_ret_entry_point) ).
+    + iModIntro; iIntros (W0 W1) "(%&%) HIW0".
+      iApply interp_monotone; last eauto; eauto.
+    + iModIntro; iIntros (W0 W1) "_ %HIW0".
+      destruct g.
+      * iApply interp_monotone_nl; last eauto; eauto.
+      * (*Trick here: value relation leads to a contradiction if p' is WL,
         since then its region cannot be permanent *)
       iDestruct ( writeLocalAllowed_valid_cap_implies with "Hvdst" ) as %Ha; eauto.
       simplify_eq.
@@ -454,10 +496,16 @@ Proof.
   unfold monotonicity_guarantees_region.
   iIntros (Hstd Hwb Hfl') "#Hvdst".
   destruct ρ;auto.
-  - destruct (isWL p') eqn: HpwlP1 ; iModIntro; simpl ; iIntros (W0 W1) "(%&%) HIW0".
-    + iApply interp_monotone; last eauto; eauto.
-    + iApply interp_monotone_nl; last eauto; eauto.
-  - iModIntro; simpl; iIntros (W0 W1) "(%&%) HIW0".
+  - destruct (isWL p') eqn: HpwlP1.
+    + iModIntro; simpl ; iIntros (W0 W1) "(%&%) HIW0".
+      iApply interp_monotone; last eauto; eauto.
+    + rewrite /future_priv_mono switcher_ret_correct.
+      rewrite decide_False //.
+      iModIntro; simpl ; iIntros (W0 W1) "% % HIW0".
+      iApply interp_monotone_nl; last eauto; eauto.
+  - rewrite /future_priv_mono switcher_ret_correct.
+    rewrite decide_False //.
+    iModIntro; simpl ; iIntros (W0 W1) "% % HIW0".
     iApply interp_monotone_nl; last eauto; eauto.
 Qed.
 
@@ -473,10 +521,17 @@ Proof.
   unfold monotonicity_guarantees_region.
   iIntros (Hstd Hwb Hfl') "#Hvdst".
   destruct ρ;auto.
-  - destruct (isWL p') eqn: HpwlP1 ; iModIntro; simpl ; iIntros (W0 W1) "(%&%) HIW0".
-    all: rewrite /interpC /safeC /= !fixpoint_interp1_eq;done.
-  - iModIntro; simpl; iIntros (W0 W1) "(%&%) HIW0".
-    all: rewrite /interpC /safeC /= !fixpoint_interp1_eq;done.
+  - destruct (isWL p') eqn: HpwlP1.
+    + iModIntro; simpl ; iIntros (W0 W1) "(%&%) HIW0".
+      rewrite /interpC /safeC /= !fixpoint_interp1_eq;done.
+    + rewrite /future_priv_mono switcher_ret_correct.
+      rewrite decide_False //.
+      iModIntro; simpl ; iIntros (W0 W1) "% % HIW0".
+      rewrite /interpC /safeC /= !fixpoint_interp1_eq;done.
+  - rewrite /future_priv_mono switcher_ret_correct.
+    rewrite decide_False //.
+    iModIntro; simpl ; iIntros (W0 W1) "% % HIW0".
+    rewrite /interpC /safeC /= !fixpoint_interp1_eq;done.
 Qed.
 
 Lemma interp_monotone_generalSd (W : WORLD) (C : CmptName) (ρ : region_type)
@@ -491,11 +546,17 @@ Proof.
   unfold monotonicity_guarantees_region.
   iIntros (Hstd Hwb Hfl') "#Hvdst".
   destruct ρ;auto.
-  - destruct (isWL p') eqn: Hpwlp' ; iModIntro; simpl; iIntros (W0 W1) "%Hrelated HIW0".
-    * iApply interp_monotone_sd; last eauto; eauto.
+  - destruct (isWL p') eqn: Hpwlp'.
+    + iModIntro; simpl; iIntros (W0 W1) "%Hrelated HIW0".
+      iApply interp_monotone_sd; last eauto; eauto.
       by apply related_sts_pub_priv_world in Hrelated.
-    * iApply interp_monotone_sd; last eauto; eauto.
-  - iModIntro; simpl; iIntros (W0 W1) "%Hrelated HIW0".
+    + rewrite /future_priv_mono switcher_ret_correct.
+      rewrite decide_False //.
+      iModIntro; simpl; iIntros (W0 W1) "%Hrelated % HIW0".
+      iApply interp_monotone_sd; last eauto; eauto.
+  - rewrite /future_priv_mono switcher_ret_correct.
+    rewrite decide_False //.
+    iModIntro; simpl; iIntros (W0 W1) "%Hrelated % HIW0".
     iApply interp_monotone_sd; last eauto; eauto.
 Qed.
 
